finish bvSgt bvSge

src/BitBlastingSimple.v
@@ -7929,7 +7929,7 @@ Qed.
 Definition bit_blast_sgt w (g: generator) (ls1 ls2 : w.+1.-tuple literal) : generator * cnf * literal :=
   bit_blast_slt g ls2 ls1.
 
-Lemma bit_blast_sgt_correct :
+Lemma bit_blast_sgt_correct_iff :
   forall w g (bs1 bs2 : BITS w.+1) E g' ls1 ls2 cs lr,
     bit_blast_sgt g ls1 ls2 = (g', cs, lr) ->
     enc_bits E ls1 bs1 ->
@@ -7944,6 +7944,85 @@ Proof.
   rewrite Hrslt; omega.
 Qed.
 
+Lemma bit_blast_sgt_correct :
+  forall w g (bs1 bs2 : BITS (w.+1)) E g' ls1 ls2 cs lr,
+    bit_blast_sgt g ls1 ls2 = (g', cs, lr) ->
+    enc_bits E ls1 bs1 ->
+    enc_bits E ls2 bs2 ->
+    interp_cnf E (add_prelude cs) ->
+    enc_bit E lr (Z.gtb (toZ bs1) (toZ bs2)).
+Proof.
+  move=> w g bs1 bs2 E g' ls1 ls2 cs lr Hslt Hl1b1 Hl2b2 HiEcs.
+  move : (bit_blast_sgt_correct_iff Hslt Hl1b1 Hl2b2 HiEcs) => H.
+  rewrite /enc_bit. apply iffBool. rewrite H Z.gt_lt_iff Z.gtb_ltb -Z.ltb_lt.
+  done.
+Qed.
+
+Definition mk_env_sgt w (E : env) g (ls1 ls2 : w.+1.-tuple literal) : env * generator * cnf * literal :=
+  mk_env_slt E g ls2 ls1.
+
+Lemma mk_env_sgt_is_bit_blast_sgt :
+  forall w E g (ls1 ls2 : w.+1.-tuple literal) E' g' cs lr,
+    mk_env_sgt E g ls1 ls2 = (E', g', cs, lr) ->
+    bit_blast_sgt g ls1 ls2 = (g', cs, lr).
+Proof.
+  move=> w E g ls1 ls2 E' g' cs lr.
+  rewrite /mk_env_sgt /bit_blast_sgt. 
+  exact: mk_env_slt_is_bit_blast_slt.
+Qed.
+
+Lemma mk_env_sgt_newer_gen :
+  forall w E g (ls1 ls2 : w.+1.-tuple literal) E' g' cs lr,
+    mk_env_sgt E g ls1 ls2 = (E', g', cs, lr) ->
+    (g <=? g')%positive.
+Proof.
+  move=> w E g ls1 ls2 E' g' cs lr. rewrite /mk_env_sgt.
+  exact: mk_env_slt_newer_gen.
+Qed.
+
+Lemma mk_env_sgt_newer_res :
+  forall w E g (ls1 ls2 : w.+1.-tuple literal) E' g' cs lr,
+    mk_env_sgt E g ls1 ls2 = (E', g', cs, lr) ->
+    newer_than_lit g' lr.
+Proof.
+  move=> w E g ls1 ls2 E' g' cs lr. rewrite /mk_env_sgt.
+  exact: mk_env_slt_newer_res.
+Qed.  
+
+Lemma mk_env_sgt_newer_cnf :
+  forall w E g (ls1 ls2 : w.+1.-tuple literal) E' g' cs lr,
+    mk_env_sgt E g ls1 ls2 = (E', g', cs, lr) ->
+    newer_than_lit g lit_tt ->
+    newer_than_lits g ls1 -> newer_than_lits g ls2 ->
+    newer_than_cnf g' cs.
+Proof.
+  move=> w E g ls1 ls2 E' g' cs lr. rewrite /mk_env_sgt.
+  move=> Hmkslt Hgt Hgl1 Hgl2.
+  exact (mk_env_slt_newer_cnf Hmkslt Hgt Hgl2 Hgl1).
+Qed.
+
+Lemma mk_env_sgt_preserve :
+  forall w E g (ls1 ls2 : w.+1.-tuple literal) E' g' cs lr,
+    mk_env_sgt E g ls1 ls2 = (E', g', cs, lr) ->
+    env_preserve E E' g.
+Proof.
+  move=> w E g ls1 ls2 E' g' cs lr. rewrite /mk_env_sgt.
+  exact: mk_env_slt_preserve.
+Qed.
+
+Lemma mk_env_sgt_sat :
+  forall w E g (ls1 ls2 : w.+1.-tuple literal) E' g' cs lr,
+    mk_env_sgt E g ls1 ls2 = (E', g', cs, lr) ->
+    newer_than_lit g lit_tt ->
+    newer_than_lits g ls1 -> newer_than_lits g ls2 ->
+    interp_cnf E' cs.
+Proof.
+  move=> w E g ls1 ls2 E' g' cs lr. rewrite /mk_env_sgt.
+  move=> Hmkslt Hgt Hgl1 Hgl2.
+  exact: (mk_env_slt_sat Hmkslt Hgt Hgl2 Hgl1).
+Qed.
+
+
 (* ===== bit_blast_sge ===== *)
 
 (*Parameter bit_blast_sge : forall w : nat, generator -> w.+1.-tuple literal -> w.+1.-tuple literal -> generator * cnf * literal.
@@ -7951,7 +8030,7 @@ Qed.
 Definition bit_blast_sge w (g: generator) (ls1 ls2 : w.+1.-tuple literal) : generator * cnf * literal :=
   bit_blast_sle g ls2 ls1.
 
-Lemma bit_blast_sge_correct :
+Lemma bit_blast_sge_correct_iff :
   forall w g (bs1 bs2 : BITS w.+1) E g' ls1 ls2 cs lr,
     bit_blast_sge g ls1 ls2 = (g', cs, lr) ->
     enc_bits E ls1 bs1 ->
@@ -7965,6 +8044,85 @@ Proof.
   move : (bit_blast_sle_correct_iff Hsle Henc2 Henc1 Hcnf) => Hrsle.
   rewrite Hrsle; omega.
 Qed.
+
+Lemma bit_blast_sge_correct :
+  forall w g (bs1 bs2 : BITS (w.+1)) E g' ls1 ls2 cs lr,
+    bit_blast_sge g ls1 ls2 = (g', cs, lr) ->
+    enc_bits E ls1 bs1 ->
+    enc_bits E ls2 bs2 ->
+    interp_cnf E (add_prelude cs) ->
+    enc_bit E lr (Z.geb (toZ bs1) (toZ bs2)).
+Proof.
+  move=> w g bs1 bs2 E g' ls1 ls2 cs lr Hslt Hl1b1 Hl2b2 HiEcs.
+  move : (bit_blast_sge_correct_iff Hslt Hl1b1 Hl2b2 HiEcs) => H.
+  rewrite /enc_bit. apply iffBool. rewrite H Z.ge_le_iff Z.geb_leb -Z.leb_le.
+  done.
+Qed.
+
+Definition mk_env_sge w (E : env) g (ls1 ls2 : w.+1.-tuple literal) : env * generator * cnf * literal :=
+  mk_env_sle E g ls2 ls1.
+
+Lemma mk_env_sge_is_bit_blast_sge :
+  forall w E g (ls1 ls2 : w.+1.-tuple literal) E' g' cs lr,
+    mk_env_sge E g ls1 ls2 = (E', g', cs, lr) ->
+    bit_blast_sge g ls1 ls2 = (g', cs, lr).
+Proof.
+  move=> w E g ls1 ls2 E' g' cs lr.
+  rewrite /mk_env_sge /bit_blast_sge. 
+  exact: mk_env_sle_is_bit_blast_sle.
+Qed.
+
+Lemma mk_env_sge_newer_gen :
+  forall w E g (ls1 ls2 : w.+1.-tuple literal) E' g' cs lr,
+    mk_env_sge E g ls1 ls2 = (E', g', cs, lr) ->
+    (g <=? g')%positive.
+Proof.
+  move=> w E g ls1 ls2 E' g' cs lr. rewrite /mk_env_sge.
+  exact: mk_env_sle_newer_gen.
+Qed.
+
+Lemma mk_env_sge_newer_res :
+  forall w E g (ls1 ls2 : w.+1.-tuple literal) E' g' cs lr,
+    mk_env_sge E g ls1 ls2 = (E', g', cs, lr) ->
+    newer_than_lit g' lr.
+Proof.
+  move=> w E g ls1 ls2 E' g' cs lr. rewrite /mk_env_sge.
+  exact: mk_env_sle_newer_res.
+Qed.  
+
+Lemma mk_env_sge_newer_cnf :
+  forall w E g (ls1 ls2 : w.+1.-tuple literal) E' g' cs lr,
+    mk_env_sge E g ls1 ls2 = (E', g', cs, lr) ->
+    newer_than_lit g lit_tt ->
+    newer_than_lits g ls1 -> newer_than_lits g ls2 ->
+    newer_than_cnf g' cs.
+Proof.
+  move=> w E g ls1 ls2 E' g' cs lr. rewrite /mk_env_sge.
+  move=> Hmksle Hgt Hgl1 Hgl2.
+  exact (mk_env_sle_newer_cnf Hmksle Hgt Hgl2 Hgl1).
+Qed.
+
+Lemma mk_env_sge_preserve :
+  forall w E g (ls1 ls2 : w.+1.-tuple literal) E' g' cs lr,
+    mk_env_sge E g ls1 ls2 = (E', g', cs, lr) ->
+    env_preserve E E' g.
+Proof.
+  move=> w E g ls1 ls2 E' g' cs lr. rewrite /mk_env_sge.
+  exact: mk_env_sle_preserve.
+Qed.
+
+Lemma mk_env_sge_sat :
+  forall w E g (ls1 ls2 : w.+1.-tuple literal) E' g' cs lr,
+    mk_env_sge E g ls1 ls2 = (E', g', cs, lr) ->
+    newer_than_lit g lit_tt ->
+    newer_than_lits g ls1 -> newer_than_lits g ls2 ->
+    interp_cnf E' cs.
+Proof.
+  move=> w E g ls1 ls2 E' g' cs lr. rewrite /mk_env_sge.
+  move=> Hmksle Hgt Hgl1 Hgl2.
+  exact: (mk_env_sle_sat Hmksle Hgt Hgl2 Hgl1).
+Qed.
+
 
 (* ===== bit_blast_lneg ===== *)
 
@@ -8283,8 +8441,16 @@ bit_blast_bexp (m : vm) (g : generator) (e : QFBV64.bexp) : vm * generator * cnf
     let '(m2, g2, cs2, ls2) := bit_blast_exp m1 g1 e2 in
     let '(gr, csr, lr) := bit_blast_sle g2 ls1 ls2 in
     (m2, gr, cs1++cs2++csr, lr)
-  | QFBV64.bvSgt w e1 e2 => (m, g, [], lit_ff) (* TODO *)
-  | QFBV64.bvSge w e1 e2 => (m, g, [], lit_ff) (* TODO *)
+  | QFBV64.bvSgt w e1 e2 => 
+    let '(m1, g1, cs1, ls1) := bit_blast_exp m g e1 in
+    let '(m2, g2, cs2, ls2) := bit_blast_exp m1 g1 e2 in
+    let '(gr, csr, lr) := bit_blast_sgt g2 ls1 ls2 in
+    (m2, gr, cs1++cs2++csr, lr)
+  | QFBV64.bvSge w e1 e2 => 
+    let '(m1, g1, cs1, ls1) := bit_blast_exp m g e1 in
+    let '(m2, g2, cs2, ls2) := bit_blast_exp m1 g1 e2 in
+    let '(gr, csr, lr) := bit_blast_sge g2 ls1 ls2 in
+    (m2, gr, cs1++cs2++csr, lr)
   | QFBV64.bvUaddo w e1 e2 => (m, g, [], lit_ff) (* TODO *)
   | QFBV64.bvUsubo w e1 e2 => (m, g, [], lit_ff) (* TODO *)
   | QFBV64.bvUmulo w e1 e2 => (m, g, [], lit_ff) (* TODO *)
@@ -8450,8 +8616,16 @@ mk_env_bexp (m : vm) (s : QFBV64.State.t) (E : env) (g : generator) (e : QFBV64.
     let '(m2, E2, g2, cs2, ls2) := mk_env_exp m1 s E1 g1 e2 in
     let '(Er, gr, csr, lr) := mk_env_sle E2 g2 ls1 ls2 in
     (m2, Er, gr, cs1++cs2++csr, lr)
-  | QFBV64.bvSgt w e1 e2 => (m, E, g, [], lit_ff) (* TODO *)
-  | QFBV64.bvSge w e1 e2 => (m, E, g, [], lit_ff) (* TODO *)
+  | QFBV64.bvSgt w e1 e2 => 
+    let '(m1, E1, g1, cs1, ls1) := mk_env_exp m s E g e1 in
+    let '(m2, E2, g2, cs2, ls2) := mk_env_exp m1 s E1 g1 e2 in
+    let '(Er, gr, csr, lr) := mk_env_sgt E2 g2 ls1 ls2 in
+    (m2, Er, gr, cs1++cs2++csr, lr)
+  | QFBV64.bvSge w e1 e2 => 
+    let '(m1, E1, g1, cs1, ls1) := mk_env_exp m s E g e1 in
+    let '(m2, E2, g2, cs2, ls2) := mk_env_exp m1 s E1 g1 e2 in
+    let '(Er, gr, csr, lr) := mk_env_sge E2 g2 ls1 ls2 in
+    (m2, Er, gr, cs1++cs2++csr, lr)
   | QFBV64.bvUaddo w e1 e2 => (m, E, g, [], lit_ff) (* TODO *)
   | QFBV64.bvUsubo w e1 e2 => (m, E, g, [], lit_ff) (* TODO *)
   | QFBV64.bvUmulo w e1 e2 => (m, E, g, [], lit_ff) (* TODO *)
@@ -8986,18 +9160,38 @@ Proof.
 Qed.
 
 Lemma bit_blast_bexp_preserve_sgt :
-  forall (w : nat) (e e0 : QFBV64.exp w) (m : vm) (g : generator)
-         (m' : vm) (g' : generator) (cs : cnf) (lrs : literal),
-    bit_blast_bexp m g (QFBV64.bvSgt w e e0) = (m', g', cs, lrs) -> vm_preserve m m'.
+  forall (w : nat) (e1 : QFBV64.exp w.+1),
+    (forall (m : vm) (g : generator)
+            (m' : vm) (g' : generator) (cs : cnf) (lrs : w.+1.-tuple literal),
+        bit_blast_exp m g e1 = (m', g', cs, lrs) -> vm_preserve m m') ->
+    forall (e2 : QFBV64.exp w.+1),
+      (forall (m : vm) (g : generator)
+              (m' : vm) (g' : generator) (cs : cnf) (lrs : w.+1.-tuple literal),
+          bit_blast_exp m g e2 = (m', g', cs, lrs) -> vm_preserve m m') ->
+      forall (m : vm) (g : generator)
+             (m' : vm) (g' : generator) (cs : cnf) (lr : literal),
+        bit_blast_bexp m g (QFBV64.bvSgt w e1 e2) = (m', g', cs, lr) ->
+        vm_preserve m m'.
 Proof.
-Admitted.
+  auto_bit_blast_vm_preserve.
+Qed.
 
 Lemma bit_blast_bexp_preserve_sge :
-  forall (w : nat) (e e0 : QFBV64.exp w) (m : vm) (g : generator)
-         (m' : vm) (g' : generator) (cs : cnf) (lrs : literal),
-    bit_blast_bexp m g (QFBV64.bvSge w e e0) = (m', g', cs, lrs) -> vm_preserve m m'.
+  forall (w : nat) (e1 : QFBV64.exp w.+1),
+    (forall (m : vm) (g : generator)
+            (m' : vm) (g' : generator) (cs : cnf) (lrs : w.+1.-tuple literal),
+        bit_blast_exp m g e1 = (m', g', cs, lrs) -> vm_preserve m m') ->
+    forall (e2 : QFBV64.exp w.+1),
+      (forall (m : vm) (g : generator)
+              (m' : vm) (g' : generator) (cs : cnf) (lrs : w.+1.-tuple literal),
+          bit_blast_exp m g e2 = (m', g', cs, lrs) -> vm_preserve m m') ->
+      forall (m : vm) (g : generator)
+             (m' : vm) (g' : generator) (cs : cnf) (lr : literal),
+        bit_blast_bexp m g (QFBV64.bvSge w e1 e2) = (m', g', cs, lr) ->
+        vm_preserve m m'.
 Proof.
-Admitted.
+  auto_bit_blast_vm_preserve.
+Qed.
 
 Lemma bit_blast_bexp_preserve_uaddo :
   forall (w : nat) (e e0 : QFBV64.exp w) (m : vm) (g : generator)
@@ -9193,8 +9387,12 @@ Proof.
   - move=> w e1 e2.
     move: (bit_blast_exp_preserve _ e1) (bit_blast_exp_preserve _ e2) => IH1 IH2.
     exact: (bit_blast_bexp_preserve_sle IH1 IH2).
-  - exact: bit_blast_bexp_preserve_sgt.
-  - exact: bit_blast_bexp_preserve_sge.
+  - move=> w e1 e2.
+    move: (bit_blast_exp_preserve _ e1) (bit_blast_exp_preserve _ e2) => IH1 IH2.
+    exact: (bit_blast_bexp_preserve_sgt IH1 IH2).
+  - move=> w e1 e2.
+    move: (bit_blast_exp_preserve _ e1) (bit_blast_exp_preserve _ e2) => IH1 IH2.
+    exact: (bit_blast_bexp_preserve_sge IH1 IH2).
   - exact: bit_blast_bexp_preserve_uaddo.
   - exact: bit_blast_bexp_preserve_usubo.
   - exact: bit_blast_bexp_preserve_umulo.
@@ -10170,26 +10368,78 @@ Proof.
 Qed.
 
 Lemma bit_blast_bexp_sgt :
-  forall (w : nat) (e e0 : QFBV64.exp w) (m : vm) (g : generator)
-         (s : QFBV64.State.t) (E : env)
-         (m' : vm) (g' : generator) (cs : cnf) (lr : literal),
-    bit_blast_bexp m g (QFBV64.bvSgt w e e0) = (m', g', cs, lr) ->
-    consistent m' E s ->
-    interp_cnf E (add_prelude cs) ->
-    enc_bit E lr (QFBV64.eval_bexp (QFBV64.bvSgt w e e0) s).
+  forall (w : nat) (e1 : QFBV64.exp w.+1),
+    (forall (m : vm) (g : generator) (s : QFBV64.State.t) (E : env)
+            (m' : vm) (g' : generator) (cs : cnf) (lrs : w.+1.-tuple literal),
+        bit_blast_exp m g e1 = (m', g', cs, lrs) ->
+        consistent m' E s ->
+        interp_cnf E (add_prelude cs) ->
+        enc_bits E lrs (QFBV64.eval_exp e1 s)) ->
+    forall (e2 : QFBV64.exp w.+1),
+      (forall (m : vm) (g : generator) (s : QFBV64.State.t) (E : env)
+              (m' : vm) (g' : generator) (cs : cnf) (lrs : w.+1.-tuple literal),
+          bit_blast_exp m g e2 = (m', g', cs, lrs) ->
+          consistent m' E s ->
+          interp_cnf E (add_prelude cs) ->
+          enc_bits E lrs (QFBV64.eval_exp e2 s)) ->
+      forall (m : vm) (g : generator) (s : QFBV64.State.t) (E : env)
+             (m' : vm) (g' : generator)
+             (cs : cnf) (lr : literal),
+        bit_blast_bexp m g (QFBV64.bvSgt w e1 e2) = (m', g', cs, lr) ->
+        consistent m' E s ->
+        interp_cnf E (add_prelude cs) ->
+        enc_bit E lr (QFBV64.eval_bexp (QFBV64.bvSgt w e1 e2) s).
 Proof.
-Admitted.
+  move=> w e1 IH1 e2 IH2 m g s E m' g' cs lr.
+  rewrite (lock interp_cnf) /= -lock.
+  case He1 : (bit_blast_exp m g e1) => [[[m1 g1] cs1] ls1].
+  case He2 : (bit_blast_exp m1 g1 e2) => [[[m2 g2] cs2] ls2].
+  case Hr : (bit_blast_sgt g2 ls1 ls2) => [[gr csr] r].
+  case=> <- _ <- <-. move=> Hcons2.
+  move: (vm_preserve_consistent (bit_blast_exp_preserve He2) Hcons2) => Hcons1.
+  move: (vm_preserve_consistent (bit_blast_exp_preserve He1) Hcons1) => Hcons0.
+  rewrite !add_prelude_append. move/andP=> [Hic1 /andP [Hic2 Hicr]].
+  apply: (bit_blast_sgt_correct Hr _ _ Hicr).
+  - exact: (IH1 _ _ _ _ _ _ _ _ He1 Hcons1 Hic1).
+  - exact: (IH2 _ _ _ _ _ _ _ _ He2 Hcons2 Hic2).
+Qed.
 
 Lemma bit_blast_bexp_sge :
-  forall (w : nat) (e e0 : QFBV64.exp w) (m : vm) (g : generator)
-         (s : QFBV64.State.t) (E : env)
-         (m' : vm) (g' : generator) (cs : cnf) (lr : literal),
-    bit_blast_bexp m g (QFBV64.bvSge w e e0) = (m', g', cs, lr) ->
-    consistent m' E s ->
-    interp_cnf E (add_prelude cs) ->
-    enc_bit E lr (QFBV64.eval_bexp (QFBV64.bvSge w e e0) s).
+  forall (w : nat) (e1 : QFBV64.exp w.+1),
+    (forall (m : vm) (g : generator) (s : QFBV64.State.t) (E : env)
+            (m' : vm) (g' : generator) (cs : cnf) (lrs : w.+1.-tuple literal),
+        bit_blast_exp m g e1 = (m', g', cs, lrs) ->
+        consistent m' E s ->
+        interp_cnf E (add_prelude cs) ->
+        enc_bits E lrs (QFBV64.eval_exp e1 s)) ->
+    forall (e2 : QFBV64.exp w.+1),
+      (forall (m : vm) (g : generator) (s : QFBV64.State.t) (E : env)
+              (m' : vm) (g' : generator) (cs : cnf) (lrs : w.+1.-tuple literal),
+          bit_blast_exp m g e2 = (m', g', cs, lrs) ->
+          consistent m' E s ->
+          interp_cnf E (add_prelude cs) ->
+          enc_bits E lrs (QFBV64.eval_exp e2 s)) ->
+      forall (m : vm) (g : generator) (s : QFBV64.State.t) (E : env)
+             (m' : vm) (g' : generator)
+             (cs : cnf) (lr : literal),
+        bit_blast_bexp m g (QFBV64.bvSge w e1 e2) = (m', g', cs, lr) ->
+        consistent m' E s ->
+        interp_cnf E (add_prelude cs) ->
+        enc_bit E lr (QFBV64.eval_bexp (QFBV64.bvSge w e1 e2) s).
 Proof.
-Admitted.
+  move=> w e1 IH1 e2 IH2 m g s E m' g' cs lr.
+  rewrite (lock interp_cnf) /= -lock.
+  case He1 : (bit_blast_exp m g e1) => [[[m1 g1] cs1] ls1].
+  case He2 : (bit_blast_exp m1 g1 e2) => [[[m2 g2] cs2] ls2].
+  case Hr : (bit_blast_sge g2 ls1 ls2) => [[gr csr] r].
+  case=> <- _ <- <-. move=> Hcons2.
+  move: (vm_preserve_consistent (bit_blast_exp_preserve He2) Hcons2) => Hcons1.
+  move: (vm_preserve_consistent (bit_blast_exp_preserve He1) Hcons1) => Hcons0.
+  rewrite !add_prelude_append. move/andP=> [Hic1 /andP [Hic2 Hicr]].
+  apply: (bit_blast_sge_correct Hr _ _ Hicr).
+  - exact: (IH1 _ _ _ _ _ _ _ _ He1 Hcons1 Hic1).
+  - exact: (IH2 _ _ _ _ _ _ _ _ He2 Hcons2 Hic2).
+Qed.
 
 Lemma bit_blast_bexp_uaddo :
   forall (w : nat) (e e0 : QFBV64.exp w) (m : vm) (g : generator)
@@ -10451,8 +10701,12 @@ Proof.
   - move=> w e1 e2.
     move: (bit_blast_exp_correct _ e1) (bit_blast_exp_correct _ e2) => IH1 IH2.
     exact: (bit_blast_bexp_sle IH1 IH2).
-  - exact: bit_blast_bexp_sgt.
-  - exact: bit_blast_bexp_sge.
+  - move=> w e1 e2.
+    move: (bit_blast_exp_correct _ e1) (bit_blast_exp_correct _ e2) => IH1 IH2.
+    exact: (bit_blast_bexp_sgt IH1 IH2).
+  - move=> w e1 e2.
+    move: (bit_blast_exp_correct _ e1) (bit_blast_exp_correct _ e2) => IH1 IH2.
+    exact: (bit_blast_bexp_sge IH1 IH2).
   - exact: bit_blast_bexp_uaddo.
   - exact: bit_blast_bexp_usubo.
   - exact: bit_blast_bexp_umulo.
@@ -11148,22 +11402,60 @@ Proof.
 Qed.
 
 Lemma mk_env_bexp_is_bit_blast_bexp_sgt :
-  forall (w : nat) (e e0 : QFBV64.exp w) (m : vm) (s : QFBV64.State.t)
-         (E : env) (g : generator) (m' : vm) (E' : env) (g' : generator)
-         (cs : cnf) (lr : literal),
-    mk_env_bexp m s E g (QFBV64.bvSgt w e e0) = (m', E', g', cs, lr) ->
-    bit_blast_bexp m g (QFBV64.bvSgt w e e0) = (m', g', cs, lr).
+  forall (w : nat) (e1 : QFBV64.exp w.+1),
+    (forall (m : vm) (E : env) (g : generator) (s : QFBV64.State.t)
+            (m' : vm) (E' : env) (g' : generator) (cs : cnf)
+            (lrs : w.+1.-tuple literal),
+        mk_env_exp m s E g e1 = (m', E', g', cs, lrs) ->
+        bit_blast_exp m g e1 = (m', g', cs, lrs)) ->
+    forall (e2 : QFBV64.exp w.+1),
+      (forall (m : vm) (E : env) (g : generator) (s : QFBV64.State.t)
+              (m' : vm) (E' : env) (g' : generator) (cs : cnf)
+              (lrs : w.+1.-tuple literal),
+          mk_env_exp m s E g e2 = (m', E', g', cs, lrs) ->
+          bit_blast_exp m g e2 = (m', g', cs, lrs)) ->
+      forall (m : vm) (s : QFBV64.State.t) (E : env) (g : generator) 
+             (m' : vm) (E' : env) (g' : generator) (cs : cnf)
+             (lr : literal),
+        mk_env_bexp m s E g (QFBV64.bvSgt w e1 e2) = (m', E', g', cs, lr) ->
+        bit_blast_bexp m g (QFBV64.bvSgt w e1 e2) = (m', g', cs, lr).
 Proof.
-Admitted.
+  move=> w e1 IH1 e2 IH2 m s E g m' E' g' cs lr /=.
+  case Hmke1 : (mk_env_exp m s E g e1) => [[[[m1 E1] g1] cs1] ls1].
+  case Hmke2 : (mk_env_exp m1 s E1 g1 e2) => [[[[m2 E2] g2] cs2] ls2].
+  case Hmkr : (mk_env_sgt E2 g2 ls1 ls2) => [[[Er gr] csr] r].
+  case=> <- _ <- <- <-.
+  rewrite (IH1 _ _ _ _ _ _ _ _ _ Hmke1) (IH2 _ _ _ _ _ _ _ _ _ Hmke2).
+  by rewrite (mk_env_sgt_is_bit_blast_sgt Hmkr).
+Qed.
 
 Lemma mk_env_bexp_is_bit_blast_bexp_sge :
-  forall (w : nat) (e e0 : QFBV64.exp w) (m : vm) (s : QFBV64.State.t)
-         (E : env) (g : generator) (m' : vm) (E' : env) (g' : generator)
-         (cs : cnf) (lr : literal),
-    mk_env_bexp m s E g (QFBV64.bvSge w e e0) = (m', E', g', cs, lr) ->
-    bit_blast_bexp m g (QFBV64.bvSge w e e0) = (m', g', cs, lr).
+  forall (w : nat) (e1 : QFBV64.exp w.+1),
+    (forall (m : vm) (E : env) (g : generator) (s : QFBV64.State.t)
+            (m' : vm) (E' : env) (g' : generator) (cs : cnf)
+            (lrs : w.+1.-tuple literal),
+        mk_env_exp m s E g e1 = (m', E', g', cs, lrs) ->
+        bit_blast_exp m g e1 = (m', g', cs, lrs)) ->
+    forall (e2 : QFBV64.exp w.+1),
+      (forall (m : vm) (E : env) (g : generator) (s : QFBV64.State.t)
+              (m' : vm) (E' : env) (g' : generator) (cs : cnf)
+              (lrs : w.+1.-tuple literal),
+          mk_env_exp m s E g e2 = (m', E', g', cs, lrs) ->
+          bit_blast_exp m g e2 = (m', g', cs, lrs)) ->
+      forall (m : vm) (s : QFBV64.State.t) (E : env) (g : generator) 
+             (m' : vm) (E' : env) (g' : generator) (cs : cnf)
+             (lr : literal),
+        mk_env_bexp m s E g (QFBV64.bvSge w e1 e2) = (m', E', g', cs, lr) ->
+        bit_blast_bexp m g (QFBV64.bvSge w e1 e2) = (m', g', cs, lr).
 Proof.
-Admitted.
+  move=> w e1 IH1 e2 IH2 m s E g m' E' g' cs lr /=.
+  case Hmke1 : (mk_env_exp m s E g e1) => [[[[m1 E1] g1] cs1] ls1].
+  case Hmke2 : (mk_env_exp m1 s E1 g1 e2) => [[[[m2 E2] g2] cs2] ls2].
+  case Hmkr : (mk_env_sge E2 g2 ls1 ls2) => [[[Er gr] csr] r].
+  case=> <- _ <- <- <-.
+  rewrite (IH1 _ _ _ _ _ _ _ _ _ Hmke1) (IH2 _ _ _ _ _ _ _ _ _ Hmke2).
+  by rewrite (mk_env_sge_is_bit_blast_sge Hmkr).
+Qed.
 
 Lemma mk_env_bexp_is_bit_blast_bexp_uaddo :
   forall (w : nat) (e e0 : QFBV64.exp w) (m : vm) (s : QFBV64.State.t)
@@ -11387,8 +11679,14 @@ Proof.
     move: (mk_env_exp_is_bit_blast_exp _ e1)
           (mk_env_exp_is_bit_blast_exp _ e2) => IH1 IH2.
     exact: (mk_env_bexp_is_bit_blast_bexp_sle IH1 IH2).
-  - exact: mk_env_bexp_is_bit_blast_bexp_sgt.
-  - exact: mk_env_bexp_is_bit_blast_bexp_sge.
+  - move=> w e1 e2.
+    move: (mk_env_exp_is_bit_blast_exp _ e1)
+          (mk_env_exp_is_bit_blast_exp _ e2) => IH1 IH2.
+    exact: (mk_env_bexp_is_bit_blast_bexp_sgt IH1 IH2).
+  - move=> w e1 e2.
+    move: (mk_env_exp_is_bit_blast_exp _ e1)
+          (mk_env_exp_is_bit_blast_exp _ e2) => IH1 IH2.
+    exact: (mk_env_bexp_is_bit_blast_bexp_sge IH1 IH2).
   - exact: mk_env_bexp_is_bit_blast_bexp_uaddo.
   - exact: mk_env_bexp_is_bit_blast_bexp_usubo.
   - exact: mk_env_bexp_is_bit_blast_bexp_umulo.
@@ -12088,22 +12386,60 @@ Proof.
 Qed.
 
 Lemma mk_env_bexp_newer_gen_sgt :
-  forall (w : nat) (e e0 : QFBV64.exp w) (m : vm) (s : QFBV64.State.t)
-         (E : env) (g : generator) (m' : vm) (E' : env) (g' : generator)
-         (cs : cnf) (lr : literal),
-    mk_env_bexp m s E g (QFBV64.bvSgt w e e0) = (m', E', g', cs, lr) ->
-    (g <=? g')%positive.
+  forall (w : nat) (e1 : QFBV64.exp w.+1),
+    (forall (m : vm) (s : QFBV64.State.t) (E : env) (g : generator)
+            (m' : vm) (E' : env) (g' : generator) (cs : cnf)
+            (lrs : w.+1.-tuple literal),
+        mk_env_exp m s E g e1 = (m', E', g', cs, lrs) -> (g <=? g')%positive) ->
+    forall (e2 : QFBV64.exp w.+1),
+      (forall (m : vm) (s : QFBV64.State.t) (E : env) (g : generator)
+              (m' : vm) (E' : env) (g' : generator) (cs : cnf)
+              (lrs : w.+1.-tuple literal),
+          mk_env_exp m s E g e2 = (m', E', g', cs, lrs) -> (g <=? g')%positive) ->
+      forall (m : vm) (s : QFBV64.State.t) (E : env) (g : generator)
+             (m' : vm) (E' : env) (g' : generator) (cs : cnf)
+             (lr : literal),
+        mk_env_bexp m s E g (QFBV64.bvSgt w e1 e2) = (m', E', g', cs, lr) ->
+        (g <=? g')%positive.
 Proof.
-Admitted.
+  move=> w e1 IH1 e2 IH2 m s E g m' E' g' cs lr /=.
+  case Hmke1 : (mk_env_exp m s E g e1) => [[[[m1 E1] g1] cs1] ls1].
+  case Hmke2 : (mk_env_exp m1 s E1 g1 e2) => [[[[m2 E2] g2] cs2] ls2].
+  case Hmkr : (mk_env_sgt E2 g2 ls1 ls2) => [[[Er gr] csr] r].
+  case=> _ _ <- _ _.
+  move: (IH1 _ _ _ _ _ _ _ _ _ Hmke1) => Hg0g1.
+  move: (IH2 _ _ _ _ _ _ _ _ _ Hmke2) => Hg1g2.
+  move: (mk_env_sgt_newer_gen Hmkr) => Hg2gr.
+  apply: (pos_leb_trans Hg0g1). apply (pos_leb_trans Hg1g2). done.
+Qed.
 
 Lemma mk_env_bexp_newer_gen_sge :
-  forall (w : nat) (e e0 : QFBV64.exp w) (m : vm) (s : QFBV64.State.t)
-         (E : env) (g : generator) (m' : vm) (E' : env) (g' : generator)
-         (cs : cnf) (lr : literal),
-    mk_env_bexp m s E g (QFBV64.bvSge w e e0) = (m', E', g', cs, lr) ->
-    (g <=? g')%positive.
+  forall (w : nat) (e1 : QFBV64.exp w.+1),
+    (forall (m : vm) (s : QFBV64.State.t) (E : env) (g : generator)
+            (m' : vm) (E' : env) (g' : generator) (cs : cnf)
+            (lrs : w.+1.-tuple literal),
+        mk_env_exp m s E g e1 = (m', E', g', cs, lrs) -> (g <=? g')%positive) ->
+    forall (e2 : QFBV64.exp w.+1),
+      (forall (m : vm) (s : QFBV64.State.t) (E : env) (g : generator)
+              (m' : vm) (E' : env) (g' : generator) (cs : cnf)
+              (lrs : w.+1.-tuple literal),
+          mk_env_exp m s E g e2 = (m', E', g', cs, lrs) -> (g <=? g')%positive) ->
+      forall (m : vm) (s : QFBV64.State.t) (E : env) (g : generator)
+             (m' : vm) (E' : env) (g' : generator) (cs : cnf)
+             (lr : literal),
+        mk_env_bexp m s E g (QFBV64.bvSge w e1 e2) = (m', E', g', cs, lr) ->
+        (g <=? g')%positive.
 Proof.
-Admitted.
+  move=> w e1 IH1 e2 IH2 m s E g m' E' g' cs lr /=.
+  case Hmke1 : (mk_env_exp m s E g e1) => [[[[m1 E1] g1] cs1] ls1].
+  case Hmke2 : (mk_env_exp m1 s E1 g1 e2) => [[[[m2 E2] g2] cs2] ls2].
+  case Hmkr : (mk_env_sge E2 g2 ls1 ls2) => [[[Er gr] csr] r].
+  case=> _ _ <- _ _.
+  move: (IH1 _ _ _ _ _ _ _ _ _ Hmke1) => Hg0g1.
+  move: (IH2 _ _ _ _ _ _ _ _ _ Hmke2) => Hg1g2.
+  move: (mk_env_sge_newer_gen Hmkr) => Hg2gr.
+  apply: (pos_leb_trans Hg0g1). apply (pos_leb_trans Hg1g2). done.
+Qed.
 
 Lemma mk_env_bexp_newer_gen_uaddo :
   forall (w : nat) (e e0 : QFBV64.exp w) (m : vm) (s : QFBV64.State.t)
@@ -12327,8 +12663,12 @@ Proof.
   - move=> w e1 e2.
     move: (mk_env_exp_newer_gen _ e1) (mk_env_exp_newer_gen _ e2) => IH1 IH2.
     exact: (mk_env_bexp_newer_gen_sle IH1 IH2).
-  - exact: mk_env_bexp_newer_gen_sgt.
-  - exact: mk_env_bexp_newer_gen_sge.
+  - move=> w e1 e2.
+    move: (mk_env_exp_newer_gen _ e1) (mk_env_exp_newer_gen _ e2) => IH1 IH2.
+    exact: (mk_env_bexp_newer_gen_sgt IH1 IH2).
+  - move=> w e1 e2.
+    move: (mk_env_exp_newer_gen _ e1) (mk_env_exp_newer_gen _ e2) => IH1 IH2.
+    exact: (mk_env_bexp_newer_gen_sge IH1 IH2).
   - exact: mk_env_bexp_newer_gen_uaddo.
   - exact: mk_env_bexp_newer_gen_usubo.
   - exact: mk_env_bexp_newer_gen_umulo.
@@ -13073,22 +13413,64 @@ Proof.
 Qed.
 
 Lemma mk_env_bexp_newer_vm_sgt :
-  forall (w : nat) (e e0 : QFBV64.exp w) (m : vm) (s : QFBV64.State.t)
-         (E : env) (g : generator) (m' : vm) (E' : env) (g' : generator)
-         (cs : cnf) (lr : literal),
-    mk_env_bexp m s E g (QFBV64.bvSgt w e e0) = (m', E', g', cs, lr) ->
-    newer_than_vm g m -> newer_than_vm g' m'.
+  forall (w : nat) (e1 : QFBV64.exp w.+1),
+    (forall (m : vm) (s : QFBV64.State.t) (E : env) (g : generator)
+            (m' : vm) (E' : env) (g' : generator) (cs : cnf)
+            (lrs : w.+1.-tuple literal),
+        mk_env_exp m s E g e1 = (m', E', g', cs, lrs) ->
+        newer_than_vm g m -> newer_than_vm g' m') ->
+    forall (e2 : QFBV64.exp w.+1),
+      (forall (m : vm) (s : QFBV64.State.t) (E : env) (g : generator)
+              (m' : vm) (E' : env) (g' : generator) (cs : cnf)
+              (lrs : w.+1.-tuple literal),
+          mk_env_exp m s E g e2 = (m', E', g', cs, lrs) ->
+          newer_than_vm g m -> newer_than_vm g' m') ->
+      forall (m : vm) (s : QFBV64.State.t) (E : env) (g : generator)
+             (m' : vm) (E' : env) (g' : generator) (cs : cnf)
+             (lr : literal),
+        mk_env_bexp m s E g (QFBV64.bvSgt w e1 e2) = (m', E', g', cs, lr) ->
+        newer_than_vm g m -> newer_than_vm g' m'.
 Proof.
-Admitted.
+  move=> w e1 IH1 e2 IH2 m s E g m' E' g' cs lr /=.
+  case Hmke1 : (mk_env_exp m s E g e1) => [[[[m1 E1] g1] cs1] ls1].
+  case Hmke2 : (mk_env_exp m1 s E1 g1 e2) => [[[[m2 E2] g2] cs2] ls2].
+  case Hmkr : (mk_env_sgt E2 g2 ls1 ls2) => [[[Er gr] csr] r].
+  case=> <- _ <- _ _ Hg0m0.
+  move: (IH1 _ _ _ _ _ _ _ _ _ Hmke1 Hg0m0) => Hg1m1.
+  move: (IH2 _ _ _ _ _ _ _ _ _ Hmke2 Hg1m1) => Hg2m2.
+  move: (mk_env_sgt_newer_gen Hmkr) => Hg2gr.
+  exact: (newer_than_vm_le_newer Hg2m2 Hg2gr).
+Qed.
 
 Lemma mk_env_bexp_newer_vm_sge :
-  forall (w : nat) (e e0 : QFBV64.exp w) (m : vm) (s : QFBV64.State.t)
-         (E : env) (g : generator) (m' : vm) (E' : env) (g' : generator)
-         (cs : cnf) (lr : literal),
-    mk_env_bexp m s E g (QFBV64.bvSge w e e0) = (m', E', g', cs, lr) ->
-    newer_than_vm g m -> newer_than_vm g' m'.
+  forall (w : nat) (e1 : QFBV64.exp w.+1),
+    (forall (m : vm) (s : QFBV64.State.t) (E : env) (g : generator)
+            (m' : vm) (E' : env) (g' : generator) (cs : cnf)
+            (lrs : w.+1.-tuple literal),
+        mk_env_exp m s E g e1 = (m', E', g', cs, lrs) ->
+        newer_than_vm g m -> newer_than_vm g' m') ->
+    forall (e2 : QFBV64.exp w.+1),
+      (forall (m : vm) (s : QFBV64.State.t) (E : env) (g : generator)
+              (m' : vm) (E' : env) (g' : generator) (cs : cnf)
+              (lrs : w.+1.-tuple literal),
+          mk_env_exp m s E g e2 = (m', E', g', cs, lrs) ->
+          newer_than_vm g m -> newer_than_vm g' m') ->
+      forall (m : vm) (s : QFBV64.State.t) (E : env) (g : generator)
+             (m' : vm) (E' : env) (g' : generator) (cs : cnf)
+             (lr : literal),
+        mk_env_bexp m s E g (QFBV64.bvSge w e1 e2) = (m', E', g', cs, lr) ->
+        newer_than_vm g m -> newer_than_vm g' m'.
 Proof.
-Admitted.
+  move=> w e1 IH1 e2 IH2 m s E g m' E' g' cs lr /=.
+  case Hmke1 : (mk_env_exp m s E g e1) => [[[[m1 E1] g1] cs1] ls1].
+  case Hmke2 : (mk_env_exp m1 s E1 g1 e2) => [[[[m2 E2] g2] cs2] ls2].
+  case Hmkr : (mk_env_sge E2 g2 ls1 ls2) => [[[Er gr] csr] r].
+  case=> <- _ <- _ _ Hg0m0.
+  move: (IH1 _ _ _ _ _ _ _ _ _ Hmke1 Hg0m0) => Hg1m1.
+  move: (IH2 _ _ _ _ _ _ _ _ _ Hmke2 Hg1m1) => Hg2m2.
+  move: (mk_env_sge_newer_gen Hmkr) => Hg2gr.
+  exact: (newer_than_vm_le_newer Hg2m2 Hg2gr).
+Qed.
 
 Lemma mk_env_bexp_newer_vm_uaddo :
   forall (w : nat) (e e0 : QFBV64.exp w) (m : vm) (s : QFBV64.State.t)
@@ -13309,8 +13691,12 @@ Proof.
   - move=> w e1 e2.
     move: (mk_env_exp_newer_vm _ e1) (mk_env_exp_newer_vm _ e2) => IH1 IH2.
     exact: (mk_env_bexp_newer_vm_sle IH1 IH2).
-  - exact: mk_env_bexp_newer_vm_sgt.
-  - exact: mk_env_bexp_newer_vm_sge.
+  - move=> w e1 e2.
+    move: (mk_env_exp_newer_vm _ e1) (mk_env_exp_newer_vm _ e2) => IH1 IH2.
+    exact: (mk_env_bexp_newer_vm_sgt IH1 IH2).
+  - move=> w e1 e2.
+    move: (mk_env_exp_newer_vm _ e1) (mk_env_exp_newer_vm _ e2) => IH1 IH2.
+    exact: (mk_env_bexp_newer_vm_sge IH1 IH2).
   - exact: mk_env_bexp_newer_vm_uaddo.
   - exact: mk_env_bexp_newer_vm_usubo.
   - exact: mk_env_bexp_newer_vm_umulo.
@@ -14031,22 +14417,34 @@ Proof.
 Qed.
 
 Lemma mk_env_bexp_newer_res_sgt :
-  forall (w : nat) (e e0 : QFBV64.exp w) (m : vm) (s : QFBV64.State.t)
+  forall (w : nat) (e1 e2 : QFBV64.exp w.+1) (m : vm) (s : QFBV64.State.t) 
          (E : env) (g : generator) (m' : vm) (E' : env) (g' : generator)
          (cs : cnf) (lr : literal),
-    mk_env_bexp m s E g (QFBV64.bvSgt w e e0) = (m', E', g', cs, lr) ->
+    mk_env_bexp m s E g (QFBV64.bvSgt w e1 e2) = (m', E', g', cs, lr) ->
     newer_than_lit g lit_tt -> newer_than_lit g' lr.
 Proof.
-Admitted.
+  move=> w e1 e2 m s E g m' E' g' cs lr /=.
+  case Hmke1 : (mk_env_exp m s E g e1) => [[[[m1 E1] g1] cs1] ls1].
+  case Hmke2 : (mk_env_exp m1 s E1 g1 e2) => [[[[m2 E2] g2] cs2] ls2].
+  case Hmkr : (mk_env_sgt E2 g2 ls1 ls2) => [[[Er gr] csr] r].
+  case=> _ _ <- _ <- Hgt.
+  exact: (mk_env_sgt_newer_res Hmkr).
+Qed.
 
 Lemma mk_env_bexp_newer_res_sge :
-  forall (w : nat) (e e0 : QFBV64.exp w) (m : vm) (s : QFBV64.State.t)
+  forall (w : nat) (e1 e2 : QFBV64.exp w.+1) (m : vm) (s : QFBV64.State.t) 
          (E : env) (g : generator) (m' : vm) (E' : env) (g' : generator)
          (cs : cnf) (lr : literal),
-    mk_env_bexp m s E g (QFBV64.bvSge w e e0) = (m', E', g', cs, lr) ->
+    mk_env_bexp m s E g (QFBV64.bvSge w e1 e2) = (m', E', g', cs, lr) ->
     newer_than_lit g lit_tt -> newer_than_lit g' lr.
 Proof.
-Admitted.
+  move=> w e1 e2 m s E g m' E' g' cs lr /=.
+  case Hmke1 : (mk_env_exp m s E g e1) => [[[[m1 E1] g1] cs1] ls1].
+  case Hmke2 : (mk_env_exp m1 s E1 g1 e2) => [[[[m2 E2] g2] cs2] ls2].
+  case Hmkr : (mk_env_sge E2 g2 ls1 ls2) => [[[Er gr] csr] r].
+  case=> _ _ <- _ <- Hgt.
+  exact: (mk_env_sge_newer_res Hmkr).
+Qed.
 
 Lemma mk_env_bexp_newer_res_uaddo :
   forall (w : nat) (e e0 : QFBV64.exp w) (m : vm) (s : QFBV64.State.t)
@@ -15378,22 +15776,110 @@ Proof.
 Qed.
 
 Lemma mk_env_bexp_newer_cnf_sgt :
-  forall (w : nat) (e e0 : QFBV64.exp w) (m : vm) (s : QFBV64.State.t)
-         (E : env) (g : generator) (m' : vm) (E' : env) (g' : generator)
-         (cs : cnf) (lr : literal),
-    mk_env_bexp m s E g (QFBV64.bvSgt w e e0) = (m', E', g', cs, lr) ->
-    newer_than_vm g m -> newer_than_lit g lit_tt -> newer_than_cnf g' cs.
+  forall (w : nat) (e1 : QFBV64.exp w.+1),
+    (forall (m : vm) (s : QFBV64.State.t) (E : env) (g : generator)
+            (m' : vm) (E' : env) (g' : generator) (cs : cnf)
+            (lrs : w.+1.-tuple literal),
+        mk_env_exp m s E g e1 = (m', E', g', cs, lrs) ->
+        newer_than_vm g m ->
+        newer_than_lit g lit_tt ->
+        newer_than_cnf g' cs) ->
+    forall (e2 : QFBV64.exp w.+1),
+      (forall (m : vm) (s : QFBV64.State.t) (E : env) (g : generator)
+              (m' : vm) (E' : env) (g' : generator) (cs : cnf)
+              (lrs : w.+1.-tuple literal),
+          mk_env_exp m s E g e2 = (m', E', g', cs, lrs) ->
+          newer_than_vm g m ->
+          newer_than_lit g lit_tt ->
+          newer_than_cnf g' cs) ->
+      forall (m : vm) (s : QFBV64.State.t) (E : env) (g : generator)
+             (m' : vm) (E' : env) (g' : generator) (cs : cnf)
+             (lr : literal),
+        mk_env_bexp m s E g (QFBV64.bvSgt w e1 e2) = (m', E', g', cs, lr) ->
+        newer_than_vm g m ->
+        newer_than_lit g lit_tt ->
+        newer_than_cnf g' cs.
 Proof.
-Admitted.
+  move=> w e1 IH1 e2 IH2 m s E g m' E' g' cs lr /=.
+  case Hmke1 : (mk_env_exp m s E g e1) => [[[[m1 E1] g1] cs1] ls1].
+  case Hmke2 : (mk_env_exp m1 s E1 g1 e2) => [[[[m2 E2] g2] cs2] ls2].
+  case Hmkr : (mk_env_sgt E2 g2 ls1 ls2) => [[[Er gr] csr] r].
+  case=> _ _ <- <- _ Hgm Hgt.
+  rewrite !newer_than_cnf_append.
+  (* newer_than_cnf gr cs1 *)
+  move: (IH1 _ _ _ _ _ _ _ _ _ Hmke1 Hgm Hgt) => Hg1c1.
+  move: (mk_env_exp_newer_gen Hmke2) => Hg1g2.
+  move: (mk_env_sgt_newer_gen Hmkr) => Hg2gr.
+  move: (newer_than_cnf_le_newer Hg1c1 (pos_leb_trans Hg1g2 Hg2gr)) => Hgrc1.
+  rewrite Hgrc1 /=.
+  (* newer_than_cnf gr cs2 *)
+  move: (mk_env_exp_newer_vm Hmke1 Hgm) => Hg1m1.
+  move: (mk_env_exp_newer_gen Hmke1) => Hgg1.
+  move: (newer_than_lit_le_newer Hgt Hgg1) => Hg1t.
+  move: (IH2 _ _ _ _ _ _ _ _ _ Hmke2 Hg1m1 Hg1t) => Hg2c2.
+  move: (newer_than_cnf_le_newer Hg2c2 Hg2gr) => Hgrc2.
+  rewrite Hgrc2 /=.
+  (* newer_than_cnf gr csr *)
+  move: (mk_env_exp_newer_res Hmke1 Hgm Hgt) => Hg1l1.
+  move: (mk_env_exp_newer_res Hmke2 Hg1m1 Hg1t) => Hg2l2.
+  move: (newer_than_lits_le_newer Hg1l1 Hg1g2) => Hg2l1.
+  move: (pos_leb_trans Hgg1 Hg1g2) => Hgg2.
+  move: (newer_than_lit_le_newer Hgt Hgg2) => Hg2t.
+  exact: (mk_env_sgt_newer_cnf Hmkr Hg2t Hg2l1 Hg2l2).
+Qed.
 
 Lemma mk_env_bexp_newer_cnf_sge :
-  forall (w : nat) (e e0 : QFBV64.exp w) (m : vm) (s : QFBV64.State.t)
-         (E : env) (g : generator) (m' : vm) (E' : env) (g' : generator)
-         (cs : cnf) (lr : literal),
-    mk_env_bexp m s E g (QFBV64.bvSge w e e0) = (m', E', g', cs, lr) ->
-    newer_than_vm g m -> newer_than_lit g lit_tt -> newer_than_cnf g' cs.
+  forall (w : nat) (e1 : QFBV64.exp w.+1),
+    (forall (m : vm) (s : QFBV64.State.t) (E : env) (g : generator)
+            (m' : vm) (E' : env) (g' : generator) (cs : cnf)
+            (lrs : w.+1.-tuple literal),
+        mk_env_exp m s E g e1 = (m', E', g', cs, lrs) ->
+        newer_than_vm g m ->
+        newer_than_lit g lit_tt ->
+        newer_than_cnf g' cs) ->
+    forall (e2 : QFBV64.exp w.+1),
+      (forall (m : vm) (s : QFBV64.State.t) (E : env) (g : generator)
+              (m' : vm) (E' : env) (g' : generator) (cs : cnf)
+              (lrs : w.+1.-tuple literal),
+          mk_env_exp m s E g e2 = (m', E', g', cs, lrs) ->
+          newer_than_vm g m ->
+          newer_than_lit g lit_tt ->
+          newer_than_cnf g' cs) ->
+      forall (m : vm) (s : QFBV64.State.t) (E : env) (g : generator)
+             (m' : vm) (E' : env) (g' : generator) (cs : cnf)
+             (lr : literal),
+        mk_env_bexp m s E g (QFBV64.bvSge w e1 e2) = (m', E', g', cs, lr) ->
+        newer_than_vm g m ->
+        newer_than_lit g lit_tt ->
+        newer_than_cnf g' cs.
 Proof.
-Admitted.
+  move=> w e1 IH1 e2 IH2 m s E g m' E' g' cs lr /=.
+  case Hmke1 : (mk_env_exp m s E g e1) => [[[[m1 E1] g1] cs1] ls1].
+  case Hmke2 : (mk_env_exp m1 s E1 g1 e2) => [[[[m2 E2] g2] cs2] ls2].
+  case Hmkr : (mk_env_sge E2 g2 ls1 ls2) => [[[Er gr] csr] r].
+  case=> _ _ <- <- _ Hgm Hgt.
+  rewrite !newer_than_cnf_append.
+  (* newer_than_cnf gr cs1 *)
+  move: (IH1 _ _ _ _ _ _ _ _ _ Hmke1 Hgm Hgt) => Hg1c1.
+  move: (mk_env_exp_newer_gen Hmke2) => Hg1g2.
+  move: (mk_env_sge_newer_gen Hmkr) => Hg2gr.
+  move: (newer_than_cnf_le_newer Hg1c1 (pos_leb_trans Hg1g2 Hg2gr)) => Hgrc1.
+  rewrite Hgrc1 /=.
+  (* newer_than_cnf gr cs2 *)
+  move: (mk_env_exp_newer_vm Hmke1 Hgm) => Hg1m1.
+  move: (mk_env_exp_newer_gen Hmke1) => Hgg1.
+  move: (newer_than_lit_le_newer Hgt Hgg1) => Hg1t.
+  move: (IH2 _ _ _ _ _ _ _ _ _ Hmke2 Hg1m1 Hg1t) => Hg2c2.
+  move: (newer_than_cnf_le_newer Hg2c2 Hg2gr) => Hgrc2.
+  rewrite Hgrc2 /=.
+  (* newer_than_cnf gr csr *)
+  move: (mk_env_exp_newer_res Hmke1 Hgm Hgt) => Hg1l1.
+  move: (mk_env_exp_newer_res Hmke2 Hg1m1 Hg1t) => Hg2l2.
+  move: (newer_than_lits_le_newer Hg1l1 Hg1g2) => Hg2l1.
+  move: (pos_leb_trans Hgg1 Hg1g2) => Hgg2.
+  move: (newer_than_lit_le_newer Hgt Hgg2) => Hg2t.
+  exact: (mk_env_sge_newer_cnf Hmkr Hg2t Hg2l1 Hg2l2).
+Qed.
 
 Lemma mk_env_bexp_newer_cnf_uaddo :
   forall (w : nat) (e e0 : QFBV64.exp w) (m : vm) (s : QFBV64.State.t)
@@ -15667,8 +16153,12 @@ Proof.
   - move=> w e1 e2.
     move: (mk_env_exp_newer_cnf _ e1) (mk_env_exp_newer_cnf _ e2) => IH1 IH2.
     exact: (mk_env_bexp_newer_cnf_sle IH1 IH2).
-  - exact: mk_env_bexp_newer_cnf_sgt.
-  - exact: mk_env_bexp_newer_cnf_sge.
+  - move=> w e1 e2.
+    move: (mk_env_exp_newer_cnf _ e1) (mk_env_exp_newer_cnf _ e2) => IH1 IH2.
+    exact: (mk_env_bexp_newer_cnf_sgt IH1 IH2).
+  - move=> w e1 e2.
+    move: (mk_env_exp_newer_cnf _ e1) (mk_env_exp_newer_cnf _ e2) => IH1 IH2.
+    exact: (mk_env_bexp_newer_cnf_sge IH1 IH2).
   - exact: mk_env_bexp_newer_cnf_uaddo.
   - exact: mk_env_bexp_newer_cnf_usubo.
   - exact: mk_env_bexp_newer_cnf_umulo.
@@ -16501,22 +16991,68 @@ Proof.
 Qed.
 
 Lemma mk_env_bexp_consistent_sgt :
-  forall (w : nat) (e e0 : QFBV64.exp w) (m : vm) (s : QFBV64.State.t)
-         (E : env) (g : generator) (m' : vm) (E' : env) (g' : generator)
-         (cs : cnf) (lr : literal),
-    mk_env_bexp m s E g (QFBV64.bvSgt w e e0) = (m', E', g', cs, lr) ->
-    newer_than_vm g m -> consistent m E s -> consistent m' E' s.
+  forall (w : nat) (e1 : QFBV64.exp w.+1),
+    (forall (m : vm) (s : QFBV64.State.t) (E : env) (g : generator)
+            (m' : vm) (E' : env) (g' : generator) (cs : cnf)
+            (lrs : w.+1.-tuple literal),
+        mk_env_exp m s E g e1 = (m', E', g', cs, lrs) ->
+        newer_than_vm g m -> consistent m E s -> consistent m' E' s) ->
+    forall (e2 : QFBV64.exp w.+1),
+      (forall (m : vm) (s : QFBV64.State.t) (E : env) (g : generator)
+              (m' : vm) (E' : env) (g' : generator) (cs : cnf)
+              (lrs : w.+1.-tuple literal),
+          mk_env_exp m s E g e2 = (m', E', g', cs, lrs) ->
+          newer_than_vm g m -> consistent m E s -> consistent m' E' s) ->
+      forall (m : vm) (s : QFBV64.State.t) (E : env) (g : generator)
+             (m' : vm) (E' : env) (g' : generator) (cs : cnf)
+             (lr : literal),
+        mk_env_bexp m s E g (QFBV64.bvSgt w e1 e2) = (m', E', g', cs, lr) ->
+        newer_than_vm g m -> consistent m E s -> consistent m' E' s.
 Proof.
-Admitted.
+  move=> w e1 IH1 e2 IH2 m s E g m' E' g' cs lr /=.
+  case Hmke1 : (mk_env_exp m s E g e1) => [[[[m1 E1] g1] cs1] ls1].
+  case Hmke2 : (mk_env_exp m1 s E1 g1 e2) => [[[[m2 E2] g2] cs2] ls2].
+  case Hmkr : (mk_env_sgt E2 g2 ls1 ls2) => [[[Er gr] csr] r].
+  case=> <- <- _ _ _ Hgm HcmE.
+  move: (IH1 _ _ _ _ _ _ _ _ _ Hmke1 Hgm HcmE) => Hcm1E1.
+  move: (mk_env_exp_newer_vm Hmke1 Hgm) => Hg1m1.
+  move: (IH2 _ _ _ _ _ _ _ _ _ Hmke2 Hg1m1 Hcm1E1) => Hcm2E2.
+  move: (mk_env_sgt_preserve Hmkr) => HpE2Er.
+  move: (mk_env_exp_newer_vm Hmke2 Hg1m1) => Hg2m2.
+  exact: (env_preserve_consistent Hg2m2 HpE2Er Hcm2E2).
+Qed.
 
 Lemma mk_env_bexp_consistent_sge :
-  forall (w : nat) (e e0 : QFBV64.exp w) (m : vm) (s : QFBV64.State.t)
-         (E : env) (g : generator) (m' : vm) (E' : env) (g' : generator)
-         (cs : cnf) (lr : literal),
-    mk_env_bexp m s E g (QFBV64.bvSge w e e0) = (m', E', g', cs, lr) ->
-    newer_than_vm g m -> consistent m E s -> consistent m' E' s.
+  forall (w : nat) (e1 : QFBV64.exp w.+1),
+    (forall (m : vm) (s : QFBV64.State.t) (E : env) (g : generator)
+            (m' : vm) (E' : env) (g' : generator) (cs : cnf)
+            (lrs : w.+1.-tuple literal),
+        mk_env_exp m s E g e1 = (m', E', g', cs, lrs) ->
+        newer_than_vm g m -> consistent m E s -> consistent m' E' s) ->
+    forall (e2 : QFBV64.exp w.+1),
+      (forall (m : vm) (s : QFBV64.State.t) (E : env) (g : generator)
+              (m' : vm) (E' : env) (g' : generator) (cs : cnf)
+              (lrs : w.+1.-tuple literal),
+          mk_env_exp m s E g e2 = (m', E', g', cs, lrs) ->
+          newer_than_vm g m -> consistent m E s -> consistent m' E' s) ->
+      forall (m : vm) (s : QFBV64.State.t) (E : env) (g : generator)
+             (m' : vm) (E' : env) (g' : generator) (cs : cnf)
+             (lr : literal),
+        mk_env_bexp m s E g (QFBV64.bvSge w e1 e2) = (m', E', g', cs, lr) ->
+        newer_than_vm g m -> consistent m E s -> consistent m' E' s.
 Proof.
-Admitted.
+  move=> w e1 IH1 e2 IH2 m s E g m' E' g' cs lr /=.
+  case Hmke1 : (mk_env_exp m s E g e1) => [[[[m1 E1] g1] cs1] ls1].
+  case Hmke2 : (mk_env_exp m1 s E1 g1 e2) => [[[[m2 E2] g2] cs2] ls2].
+  case Hmkr : (mk_env_sge E2 g2 ls1 ls2) => [[[Er gr] csr] r].
+  case=> <- <- _ _ _ Hgm HcmE.
+  move: (IH1 _ _ _ _ _ _ _ _ _ Hmke1 Hgm HcmE) => Hcm1E1.
+  move: (mk_env_exp_newer_vm Hmke1 Hgm) => Hg1m1.
+  move: (IH2 _ _ _ _ _ _ _ _ _ Hmke2 Hg1m1 Hcm1E1) => Hcm2E2.
+  move: (mk_env_sge_preserve Hmkr) => HpE2Er.
+  move: (mk_env_exp_newer_vm Hmke2 Hg1m1) => Hg2m2.
+  exact: (env_preserve_consistent Hg2m2 HpE2Er Hcm2E2).
+Qed.
 
 Lemma mk_env_bexp_consistent_uaddo :
   forall (w : nat) (e e0 : QFBV64.exp w) (m : vm) (s : QFBV64.State.t)
@@ -16754,8 +17290,12 @@ Proof.
   - move=> w e1 e2.
     move: (mk_env_exp_consistent _ e1) (mk_env_exp_consistent _ e2) => IH1 IH2.
     exact: (mk_env_bexp_consistent_sle IH1 IH2).
-  - exact: mk_env_bexp_consistent_sgt.
-  - exact: mk_env_bexp_consistent_sge.
+  - move=> w e1 e2.
+    move: (mk_env_exp_consistent _ e1) (mk_env_exp_consistent _ e2) => IH1 IH2.
+    exact: (mk_env_bexp_consistent_sgt IH1 IH2).
+  - move=> w e1 e2.
+    move: (mk_env_exp_consistent _ e1) (mk_env_exp_consistent _ e2) => IH1 IH2.
+    exact: (mk_env_bexp_consistent_sge IH1 IH2).
   - exact: mk_env_bexp_consistent_uaddo.
   - exact: mk_env_bexp_consistent_usubo.
   - exact: mk_env_bexp_consistent_umulo.
@@ -17538,22 +18078,68 @@ Proof.
 Qed.
 
 Lemma mk_env_bexp_preserve_sgt :
-  forall (w : nat) (e e0 : QFBV64.exp w) (m : vm) (s : QFBV64.State.t)
-         (E : env) (g : generator) (m' : vm) (E' : env) (g' : generator)
-         (cs : cnf) (lr : literal),
-    mk_env_bexp m s E g (QFBV64.bvSgt w e e0) = (m', E', g', cs, lr) ->
-    env_preserve E E' g.
+  forall (w : nat) (e1 : QFBV64.exp w.+1),
+    (forall (m : vm) (s : QFBV64.State.t) (E : env) (g : generator)
+            (m' : vm) (E' : env) (g' : generator) (cs : cnf)
+            (lrs : w.+1.-tuple literal),
+        mk_env_exp m s E g e1 = (m', E', g', cs, lrs) -> env_preserve E E' g) ->
+    forall (e2 : QFBV64.exp w.+1),
+      (forall (m : vm) (s : QFBV64.State.t) (E : env) (g : generator)
+              (m' : vm) (E' : env) (g' : generator) (cs : cnf)
+              (lrs : w.+1.-tuple literal),
+          mk_env_exp m s E g e2 = (m', E', g', cs, lrs) -> env_preserve E E' g) ->
+      forall (m : vm) (s : QFBV64.State.t) (E : env) (g : generator)
+             (m' : vm) (E' : env) (g' : generator) (cs : cnf)
+             (lr : literal),
+        mk_env_bexp m s E g (QFBV64.bvSgt w e1 e2) = (m', E', g', cs, lr) ->
+        env_preserve E E' g.
 Proof.
-Admitted.
+  move=> w e1 IH1 e2 IH2 m s E g m' E' g' cs lr /=.
+  case Hmke1 : (mk_env_exp m s E g e1) => [[[[m1 E1] g1] cs1] ls1].
+  case Hmke2 : (mk_env_exp m1 s E1 g1 e2) => [[[[m2 E2] g2] cs2] ls2].
+  case Hmkr : (mk_env_sgt E2 g2 ls1 ls2) => [[[Er gr] csr] r].
+  case=> _ <- _ _ _.
+  move: (IH1 _ _ _ _ _ _ _ _ _ Hmke1) => HpEE1g.
+  move: (IH2 _ _ _ _ _ _ _ _ _ Hmke2) => HpE1E2g1.
+  move: (mk_env_sgt_preserve Hmkr) => HpE2Erg2.
+  move: (mk_env_exp_newer_gen Hmke1) (mk_env_exp_newer_gen Hmke2) => Hgg1 Hg1g2.
+  move: (env_preserve_le HpE1E2g1 Hgg1) => HpE1E2g.
+  move: (env_preserve_le HpE2Erg2 (pos_leb_trans Hgg1 Hg1g2)) => HpE2Erg.
+  apply: (env_preserve_trans _ HpE2Erg).
+  exact: (env_preserve_trans HpEE1g HpE1E2g).
+Qed.
 
 Lemma mk_env_bexp_preserve_sge :
-  forall (w : nat) (e e0 : QFBV64.exp w) (m : vm) (s : QFBV64.State.t)
-         (E : env) (g : generator) (m' : vm) (E' : env) (g' : generator)
-         (cs : cnf) (lr : literal),
-    mk_env_bexp m s E g (QFBV64.bvSge w e e0) = (m', E', g', cs, lr) ->
-    env_preserve E E' g.
+  forall (w : nat) (e1 : QFBV64.exp w.+1),
+    (forall (m : vm) (s : QFBV64.State.t) (E : env) (g : generator)
+            (m' : vm) (E' : env) (g' : generator) (cs : cnf)
+            (lrs : w.+1.-tuple literal),
+        mk_env_exp m s E g e1 = (m', E', g', cs, lrs) -> env_preserve E E' g) ->
+    forall (e2 : QFBV64.exp w.+1),
+      (forall (m : vm) (s : QFBV64.State.t) (E : env) (g : generator)
+              (m' : vm) (E' : env) (g' : generator) (cs : cnf)
+              (lrs : w.+1.-tuple literal),
+          mk_env_exp m s E g e2 = (m', E', g', cs, lrs) -> env_preserve E E' g) ->
+      forall (m : vm) (s : QFBV64.State.t) (E : env) (g : generator)
+             (m' : vm) (E' : env) (g' : generator) (cs : cnf)
+             (lr : literal),
+        mk_env_bexp m s E g (QFBV64.bvSge w e1 e2) = (m', E', g', cs, lr) ->
+        env_preserve E E' g.
 Proof.
-Admitted.
+  move=> w e1 IH1 e2 IH2 m s E g m' E' g' cs lr /=.
+  case Hmke1 : (mk_env_exp m s E g e1) => [[[[m1 E1] g1] cs1] ls1].
+  case Hmke2 : (mk_env_exp m1 s E1 g1 e2) => [[[[m2 E2] g2] cs2] ls2].
+  case Hmkr : (mk_env_sge E2 g2 ls1 ls2) => [[[Er gr] csr] r].
+  case=> _ <- _ _ _.
+  move: (IH1 _ _ _ _ _ _ _ _ _ Hmke1) => HpEE1g.
+  move: (IH2 _ _ _ _ _ _ _ _ _ Hmke2) => HpE1E2g1.
+  move: (mk_env_sge_preserve Hmkr) => HpE2Erg2.
+  move: (mk_env_exp_newer_gen Hmke1) (mk_env_exp_newer_gen Hmke2) => Hgg1 Hg1g2.
+  move: (env_preserve_le HpE1E2g1 Hgg1) => HpE1E2g.
+  move: (env_preserve_le HpE2Erg2 (pos_leb_trans Hgg1 Hg1g2)) => HpE2Erg.
+  apply: (env_preserve_trans _ HpE2Erg).
+  exact: (env_preserve_trans HpEE1g HpE1E2g).
+Qed.
 
 Lemma mk_env_bexp_preserve_uaddo :
   forall (w : nat) (e e0 : QFBV64.exp w) (m : vm) (s : QFBV64.State.t)
@@ -17789,8 +18375,12 @@ Proof.
   - move=> w e1 e2.
     move: (mk_env_exp_preserve _ e1) (mk_env_exp_preserve _ e2) => IH1 IH2.
     exact: (mk_env_bexp_preserve_sle IH1 IH2).
-  - exact: mk_env_bexp_preserve_sgt.
-  - exact: mk_env_bexp_preserve_sge.
+  - move=> w e1 e2.
+    move: (mk_env_exp_preserve _ e1) (mk_env_exp_preserve _ e2) => IH1 IH2.
+    exact: (mk_env_bexp_preserve_sgt IH1 IH2).
+  - move=> w e1 e2.
+    move: (mk_env_exp_preserve _ e1) (mk_env_exp_preserve _ e2) => IH1 IH2.
+    exact: (mk_env_bexp_preserve_sge IH1 IH2).
   - exact: mk_env_bexp_preserve_uaddo.
   - exact: mk_env_bexp_preserve_usubo.
   - exact: mk_env_bexp_preserve_umulo.
@@ -19056,22 +19646,100 @@ Proof.
 Qed.
 
 Lemma mk_env_bexp_sat_sgt :
-  forall (w : nat) (e e0 : QFBV64.exp w) (m : vm) (s : QFBV64.State.t)
-         (E : env) (g : generator) (m' : vm) (E' : env) (g' : generator)
-         (cs : cnf) (lr : literal),
-    mk_env_bexp m s E g (QFBV64.bvSgt w e e0) = (m', E', g', cs, lr) ->
-    newer_than_vm g m -> newer_than_lit g lit_tt -> interp_cnf E' cs.
+  forall (w : nat) (e1 : QFBV64.exp w.+1),
+    (forall (m : vm) (s : QFBV64.State.t) (E : env) (g : generator)
+            (m' : vm) (E' : env) (g' : generator) (cs : cnf)
+            (lrs : w.+1.-tuple literal),
+        mk_env_exp m s E g e1 = (m', E', g', cs, lrs) ->
+        newer_than_vm g m -> newer_than_lit g lit_tt -> interp_cnf E' cs) ->
+    forall (e2 : QFBV64.exp w.+1),
+      (forall (m : vm) (s : QFBV64.State.t) (E : env) (g : generator)
+              (m' : vm) (E' : env) (g' : generator) (cs : cnf)
+              (lrs : w.+1.-tuple literal),
+          mk_env_exp m s E g e2 = (m', E', g', cs, lrs) ->
+          newer_than_vm g m -> newer_than_lit g lit_tt -> interp_cnf E' cs) ->
+      forall (m : vm) (s : QFBV64.State.t) (E : env) (g : generator)
+             (m' : vm) (E' : env) (g' : generator) (cs : cnf)
+             (lr : literal),
+        mk_env_bexp m s E g (QFBV64.bvSgt w e1 e2) = (m', E', g', cs, lr) ->
+        newer_than_vm g m -> newer_than_lit g lit_tt -> interp_cnf E' cs.
 Proof.
-Admitted.
+  move=> w e1 IH1 e2 IH2 m s E g m' E' g' cs lr /=.
+  case Hmke1 : (mk_env_exp m s E g e1) => [[[[m1 E1] g1] cs1] ls1].
+  case Hmke2 : (mk_env_exp m1 s E1 g1 e2) => [[[[m2 E2] g2] cs2] ls2].
+  case Hmkr : (mk_env_sgt E2 g2 ls1 ls2) => [[[Er gr] csr] r].
+  case=> _ <- _ <- _ Hgm Hgt. rewrite !interp_cnf_append.
+  (* interp_cnf Er cs1 *)
+  move: (IH1 _ _ _ _ _ _ _ _ _ Hmke1 Hgm Hgt) => HiE1c1.
+  move: (mk_env_exp_preserve Hmke2) => HpE1E2g1.
+  move: (mk_env_sgt_preserve Hmkr) => HpE2Erg2.
+  move: (mk_env_exp_newer_gen Hmke2) => Hg1g2.
+  move: (env_preserve_le HpE2Erg2 Hg1g2) => HpE2Erg1.
+  move: (env_preserve_trans HpE1E2g1 HpE2Erg1) => HpE1Erg1.
+  move: (mk_env_exp_newer_cnf Hmke1 Hgm Hgt) => Hg1c1.
+  rewrite (env_preserve_cnf HpE1Erg1 Hg1c1) HiE1c1 /=.
+  (* interp_cnf Er cs2 *)
+  move: (mk_env_exp_newer_vm Hmke1 Hgm) => Hg1m1.
+  move: (mk_env_exp_newer_gen Hmke1) => Hgg1.
+  move: (newer_than_lit_le_newer Hgt Hgg1) => Hg1t.
+  move: (IH2 _ _ _ _ _ _ _ _ _ Hmke2 Hg1m1 Hg1t) => HiE2c2.
+  move: (mk_env_exp_newer_cnf Hmke2 Hg1m1 Hg1t) => Hg2c2.
+  rewrite (env_preserve_cnf HpE2Erg2 Hg2c2) HiE2c2 /=.
+  (* interp_cnf Er csr *)
+  move: (mk_env_exp_newer_res Hmke1 Hgm Hgt) => Hg1l1.
+  move: (mk_env_exp_newer_res Hmke2 Hg1m1 Hg1t) => Hg2l2.
+  move: (newer_than_lits_le_newer Hg1l1 Hg1g2) => Hg2l1.
+  move: (newer_than_lit_le_newer Hg1t Hg1g2) => Hg2t.
+  exact: (mk_env_sgt_sat Hmkr Hg2t Hg2l1 Hg2l2).
+Qed.
 
 Lemma mk_env_bexp_sat_sge :
-  forall (w : nat) (e e0 : QFBV64.exp w) (m : vm) (s : QFBV64.State.t)
-         (E : env) (g : generator) (m' : vm) (E' : env) (g' : generator)
-         (cs : cnf) (lr : literal),
-    mk_env_bexp m s E g (QFBV64.bvSge w e e0) = (m', E', g', cs, lr) ->
-    newer_than_vm g m -> newer_than_lit g lit_tt -> interp_cnf E' cs.
+  forall (w : nat) (e1 : QFBV64.exp w.+1),
+    (forall (m : vm) (s : QFBV64.State.t) (E : env) (g : generator)
+            (m' : vm) (E' : env) (g' : generator) (cs : cnf)
+            (lrs : w.+1.-tuple literal),
+        mk_env_exp m s E g e1 = (m', E', g', cs, lrs) ->
+        newer_than_vm g m -> newer_than_lit g lit_tt -> interp_cnf E' cs) ->
+    forall (e2 : QFBV64.exp w.+1),
+      (forall (m : vm) (s : QFBV64.State.t) (E : env) (g : generator)
+              (m' : vm) (E' : env) (g' : generator) (cs : cnf)
+              (lrs : w.+1.-tuple literal),
+          mk_env_exp m s E g e2 = (m', E', g', cs, lrs) ->
+          newer_than_vm g m -> newer_than_lit g lit_tt -> interp_cnf E' cs) ->
+      forall (m : vm) (s : QFBV64.State.t) (E : env) (g : generator)
+             (m' : vm) (E' : env) (g' : generator) (cs : cnf)
+             (lr : literal),
+        mk_env_bexp m s E g (QFBV64.bvSge w e1 e2) = (m', E', g', cs, lr) ->
+        newer_than_vm g m -> newer_than_lit g lit_tt -> interp_cnf E' cs.
 Proof.
-Admitted.
+  move=> w e1 IH1 e2 IH2 m s E g m' E' g' cs lr /=.
+  case Hmke1 : (mk_env_exp m s E g e1) => [[[[m1 E1] g1] cs1] ls1].
+  case Hmke2 : (mk_env_exp m1 s E1 g1 e2) => [[[[m2 E2] g2] cs2] ls2].
+  case Hmkr : (mk_env_sge E2 g2 ls1 ls2) => [[[Er gr] csr] r].
+  case=> _ <- _ <- _ Hgm Hgt. rewrite !interp_cnf_append.
+  (* interp_cnf Er cs1 *)
+  move: (IH1 _ _ _ _ _ _ _ _ _ Hmke1 Hgm Hgt) => HiE1c1.
+  move: (mk_env_exp_preserve Hmke2) => HpE1E2g1.
+  move: (mk_env_sge_preserve Hmkr) => HpE2Erg2.
+  move: (mk_env_exp_newer_gen Hmke2) => Hg1g2.
+  move: (env_preserve_le HpE2Erg2 Hg1g2) => HpE2Erg1.
+  move: (env_preserve_trans HpE1E2g1 HpE2Erg1) => HpE1Erg1.
+  move: (mk_env_exp_newer_cnf Hmke1 Hgm Hgt) => Hg1c1.
+  rewrite (env_preserve_cnf HpE1Erg1 Hg1c1) HiE1c1 /=.
+  (* interp_cnf Er cs2 *)
+  move: (mk_env_exp_newer_vm Hmke1 Hgm) => Hg1m1.
+  move: (mk_env_exp_newer_gen Hmke1) => Hgg1.
+  move: (newer_than_lit_le_newer Hgt Hgg1) => Hg1t.
+  move: (IH2 _ _ _ _ _ _ _ _ _ Hmke2 Hg1m1 Hg1t) => HiE2c2.
+  move: (mk_env_exp_newer_cnf Hmke2 Hg1m1 Hg1t) => Hg2c2.
+  rewrite (env_preserve_cnf HpE2Erg2 Hg2c2) HiE2c2 /=.
+  (* interp_cnf Er csr *)
+  move: (mk_env_exp_newer_res Hmke1 Hgm Hgt) => Hg1l1.
+  move: (mk_env_exp_newer_res Hmke2 Hg1m1 Hg1t) => Hg2l2.
+  move: (newer_than_lits_le_newer Hg1l1 Hg1g2) => Hg2l1.
+  move: (newer_than_lit_le_newer Hg1t Hg1g2) => Hg2t.
+  exact: (mk_env_sge_sat Hmkr Hg2t Hg2l1 Hg2l2).
+Qed.
 
 Lemma mk_env_bexp_sat_uaddo :
   forall (w : nat) (e e0 : QFBV64.exp w) (m : vm) (s : QFBV64.State.t)
@@ -19343,8 +20011,12 @@ Proof.
   - move=> w e1 e2.
     move: (mk_env_exp_sat _ e1) (mk_env_exp_sat _ e2) => IH1 IH2.
     exact: (mk_env_bexp_sat_sle IH1 IH2).
-  - exact: mk_env_bexp_sat_sgt.
-  - exact: mk_env_bexp_sat_sge.
+  - move=> w e1 e2.
+    move: (mk_env_exp_sat _ e1) (mk_env_exp_sat _ e2) => IH1 IH2.
+    exact: (mk_env_bexp_sat_sgt IH1 IH2).
+  - move=> w e1 e2.
+    move: (mk_env_exp_sat _ e1) (mk_env_exp_sat _ e2) => IH1 IH2.
+    exact: (mk_env_bexp_sat_sge IH1 IH2).
   - exact: mk_env_bexp_sat_uaddo.
   - exact: mk_env_bexp_sat_usubo.
   - exact: mk_env_bexp_sat_umulo.
